Filled some Gaps in basic Def.s

ExistentialRules/ChaseSequence/Termination/Linear.lean
@@ -6,6 +6,7 @@ section Rules
 
   def Rule.isLinear (rule : Rule sig) : Prop := rule.body.length = 1 -- maybe this should be ≤ 1 but equality makes things more elegant for now
   def Rule.exactlyTwoHeadAtoms (rule : Rule sig) (det : rule.isDeterministic) : Prop := (rule.head[0]'(by simp only [isDeterministic, decide_eq_true_iff] at det; simp [det])).length = 2
+  --general rules in (AtomsAndFacts.Basic) allow lists of conjunctions in their head (instead of just cunjunctions of atoms), this is why the above def. is so complicated
 
   -- in the context of the target paper, linear rules have the following properties
   structure LinearRule (sig : Signature) [DecidableEq sig.P] [DecidableEq sig.C] [DecidableEq sig.V] where
@@ -19,7 +20,7 @@ section Rules
     def body (rule : LinearRule sig) : FunctionFreeAtom sig := rule.rule.body[0]'(by have linear := rule.linear; simp only [Rule.isLinear] at linear; simp [linear])
     def head (rule : LinearRule sig) : FunctionFreeAtom sig × FunctionFreeAtom sig :=
       let conj := rule.rule.head[0]'(by have det := rule.deterministic; simp only [Rule.isDeterministic, decide_eq_true_iff] at det; simp [det])
-      have length_conj : conj.length = 2 := by sorry
+      have length_conj : conj.length = 2 := by have twohead := rule.exactlyTwoHeadAtoms; simp only [Rule.exactlyTwoHeadAtoms] at twohead; simp[conj,twohead];
       (conj[0], conj[1])
 
   end LinearRule
@@ -33,9 +34,35 @@ end Rules
 
 section SubstitutionsAndTriggers
 
+  def extend_Substitutution  (s: GroundSubstitution sig) (v: sig.V) (c: GroundTerm sig) : GroundSubstitution sig := fun x => if x = v then c else s x
+
+  def matchVarorCons (s: GroundSubstitution sig) (t : VarOrConst sig) (gt : GroundTerm sig)(vars : List (sig.V)) : Option (GroundSubstitution sig) :=
+    match t with
+      | .const c => if gt = GroundTerm.const c then Option.some s else Option.none
+      | .var v =>
+          if v ∈ vars -- Varas ist liste von variablen, die schon eine zuordnung in s haben
+          then if gt = s v then Option.some s else Option.none--triit auf, wenn es für v schon eine andere substitution gab
+          else some (extend_Substitutution s v gt)
+
+  def matchTermList (s: GroundSubstitution sig) (vars : List (sig.V)) (l : List ((VarOrConst sig) × (GroundTerm sig))) : Option (GroundSubstitution sig) :=
+    match l with
+    | .nil => Option.some s
+    | (t, gt) :: ls =>
+      have s' := matchVarorCons s t gt vars
+      match s' with
+      |Option.none => Option.none
+      |Option.some s' =>
+        match t with
+        | .var v => matchTermList s' (v::vars) ls
+        | .const _ => matchTermList s' vars ls
+
   -- The paper just calles this a homomorphism but we call this special kind of homomorphism a (ground) substitution.
   -- This will require auxiliary definitions.
-  def GroundSubstitution.from_atom_and_fact (atom : FunctionFreeAtom sig) (fact : Fact sig) : Option (GroundSubstitution sig) := sorry
+  def GroundSubstitution.from_atom_and_fact (atom : FunctionFreeAtom sig) (fact : Fact sig) : Option (GroundSubstitution sig) :=
+    if atom.predicate = fact.predicate
+    then matchTermList (some s) List.nil (List.zip atom.terms fact.terms)  --> wie kann ich die substiution initial definieren?
+    else Option.none
+
 
   theorem GroundSubstitution.apply_function_free_atom_from_atom_and_fact {atom : FunctionFreeAtom sig} {fact : Fact sig} :
       ∀ subs, (GroundSubstitution.from_atom_and_fact atom fact) = some subs -> subs.apply_function_free_atom atom = fact := by
@@ -51,23 +78,57 @@ section SubstitutionsAndTriggers
       subs := subs
     })
 
+  theorem PreTrigger.from_rule_and_fact_some_implies {rule : LinearRule sig} {fact : Fact sig} :
+      ∀ {trg}, PreTrigger.from_rule_and_fact rule fact = some trg → trg.rule = rule.rule ∧ GroundSubstitution.from_atom_and_fact rule.body fact = some trg.subs := by
+        unfold PreTrigger.from_rule_and_fact;
+        cases PreTrigger.from_rule_and_fact rule fact;
+        repeat simp;
+
+
   -- this is definition 6 but we do not need the address u
   -- we use the already existing (Pre)Triggers to define the actual result of the rule application
   def ruleApply (rule : LinearRule sig) (fact : Fact sig) : Option (Fact sig × Fact sig) :=
-    (PreTrigger.from_rule_and_fact rule fact).map (fun trg =>
+    (PreTrigger.from_rule_and_fact rule fact).attach.map (fun ⟨trg, trg_orig⟩ =>
+      have h:= And.left (PreTrigger.from_rule_and_fact_some_implies trg_orig);
+      have det := rule.deterministic;
       let mapped_head : List (List (Fact sig)) := trg.mapped_head
-      have length_mapped_head : mapped_head.length = 1 := by simp only [mapped_head, PreTrigger.length_mapped_head]; sorry
+      have length_mapped_head : mapped_head.length = 1 := by
+        simp only [mapped_head, PreTrigger.length_mapped_head];
+        rw[h]
+        simp [Rule.isDeterministic] at det;
+        exact det;
       let conj := mapped_head[0]
-      have length_conj : conj.length = 2 := by sorry
+      have length_conj : conj.length = 2 := by
+        simp only [mapped_head, conj];
+        have h2 := (PreTrigger.length_each_mapped_head trg 0);
+          simp[mapped_head, length_mapped_head] at h2;
+          simp [Rule.isDeterministic] at det; simp[h, det] at h2;
+          rw[h2];
+          have twohead := rule.exactlyTwoHeadAtoms; simp only [Rule.exactlyTwoHeadAtoms] at twohead;
+          simp[twohead];
       (conj[0], conj[1])
     )
 
   -- This allows us to take a bit of a shortcut when we try to unfold the ruleApply definition in proofs.
   -- We could also use this for the definition instead but the above should be more canonical.
   theorem ruleApply_eq {rule : LinearRule sig} {fact : Fact sig} :
-      let trg_opt := PreTrigger.from_rule_and_fact rule fact
+      let trg_opt := (PreTrigger.from_rule_and_fact rule fact)
       ruleApply rule fact = trg_opt.map (fun trg => (trg.apply_to_function_free_atom 0 rule.head.fst, trg.apply_to_function_free_atom 0 rule.head.snd)) := by
-    sorry
+      intro tr;
+      rw[ruleApply];
+      have htr : PreTrigger.from_rule_and_fact rule fact = tr := rfl;
+      rcases tr ;
+      -- case none
+      simp;
+      rw[htr];
+      --case some
+      simp;
+      simp [PreTrigger.mapped_head];
+      simp[LinearRule.head];
+      expose_names;
+      exists val;
+      exists htr;
+      simp[And.left (PreTrigger.from_rule_and_fact_some_implies htr)];
 
 end SubstitutionsAndTriggers
 
@@ -84,12 +145,28 @@ section Addresses
   -- NOTE: Maybe an inductive definition with multiple cases would be more useful here, not sure yet...
   structure Address (fs : FactSet sig) (rs : LinearRuleSet sig) where
     initialAtom : {f : Fact sig // f ∈ fs}
-    path : List {sym : AddressSymbol sig // sym ∈ addressSymbols rs}
+    path : List {sym : AddressSymbol sig // sym ∈ addressSymbols rs} --Frage: wie herum die liste besser füllen? (in lesrichtung, oder so, dass das neue elem. immer vorne drangehängt wird)
+
+
+/-
+  def all_prefix_addresses_in_set {fs: FactSet sig} (a: Address fs rs) (f: Set (Address fs rs)) : Prop :=
+    match a.path with
+    |[] => true
+    |list => let b:= {a with path := list.dropLastTR}; b ∈ f ∧ all_prefix_addresses_in_set b f
+ -/
+
+ -- with this definition, we use the List of address-symbols that bulids the path from rigth to left (contrary on how it's written in the paper)
+ -- therefore we would write an address wuv ∈ IA* (with w ∈ I, u,v ∈ A) as {initialAtom := w , path :=[v,u]}
+  def immed_prefix_address_in_set {fs: FactSet sig} (a: Address fs rs) (f : Set (Address fs rs)) : Prop :=
+    match a.path with
+    |[] => true
+    |_::ls => let b:= {a with path := ls}; b ∈ f
+
 
   structure Forest (fs : FactSet sig) (rs : LinearRuleSet sig) where
     f : Set (Address fs rs)
-    fs_contained : sorry -- fs shall be contained in f (this should likely involve auxiliary definitions)
-    isPrefixClosed : sorry
+    fs_contained : ∀ fact ∈ fs, ∃ a ∈ f , fact = a.initialAtom ∧ a.path = []  -- fs shall be contained in f (this should likely involve auxiliary definitions)
+    isPrefixClosed : ∀ a ∈ f, immed_prefix_address_in_set a f --as we enforce this check on all a ∈ f, we only need to veryfy that it's immediate predecessor is in f as well
 
 end Addresses
 
@@ -99,5 +176,14 @@ section ObvliviousChaseRepresentation
   -- Maybe we need to discuss this as it might not be quite obvious how to do it.
   -- I think the idea would be to first define the labelling function returning an option and then to define the oblivious chase representation as the forest of all addresses where the labelling function returns some ... on each address.
 
-end ObvliviousChaseRepresentation
+  def labellingFunction {rs: LinearRuleSet sig} (w : Address fs rs) : Option (Fact sig) :=
+    match w.path with
+    |[] => w.initialAtom
+    |r::u =>
+      let lu := labellingFunction {w with path := u};
+      match lu with
+      |Option.none => Option.none
+      |some lu => (ruleApply r.rule lu ).map (fun x => if r.headIndex = 0 then x.fst else x.snd) --wie kann ich hier zeigen, dass u : AddressSymbol ist? --
 
+
+end ObvliviousChaseRepresentation
